add Verifications & method move

Drone.dfy
@@ -2,119 +2,187 @@
     Handout 2
 
 */
-
-class Point{
-
-    var x:real;
-    var y:real;
-    var z:real;
-
-    constructor(x:real, y:real, z:real) 
-    {
-        this.x := x;
-        this.y := y;
-        this.z := z;
-    
-    }
-
-    method getX() returns (x:real)
-    {
-        return x;
-    }
-
-    method getY() returns (y:real){
-        return y;
-    }
-
-    method getZ() returns (z:real){
-        return z;
-    }
-
-}
    
 class Drone {
     // r -> radius
     // n -> operation height
-    var r:real;
-    
-    var n:real;
+    var r:int;
+    var n:int;
+    var x:int;
+    var targetX:int;
+    var y:int;
+    var targetY:int;
+    var z:int;
+    var targetZ:int;
+
+    var points:seq<(int, int, int)>;
+
 
 
     var curSpeed:int;
+    var maxSpeed:int;
 
-    var curPosition:Point;
 
-    var point:Point;
-    var wayPoints:array<Point>;
 
-    constructor() 
+    constructor(r:int, n:int) 
+    requires r > 0 && n > 0
+    ensures RepInv()
     {
     
-        this.r := 0.0;
-        this.n := 0.0;
+        this.r := r;
+        this.n := n;
+        this.x := 0;
+        this.y := 0;
+        this.z := 0;
         this.curSpeed := 0;
-        this.wayPoints := new array<Point>;
-        this.curPosition := new Point(0.0,0.0,0.0);
+        this.maxSpeed := 10;
+        this.points := [];
+        
 
         
     }
 
     function RepInv():bool
-    reads this`r ,this`n, 
+     reads this`x, this`y, this`z, this`r, this`n, this`curSpeed, this`maxSpeed
     {
+        //verify speed
+        0 <= curSpeed <= maxSpeed 
 
+        && 
+        
+        0 <= r && 0 <= n
+
+        &&
+
+        verifyBoundaries(x,y,z)
+        
+        
+    }
+
+    function verifyBoundaries(x:int, y:int, z:int) : bool
+    reads this`r, this`n
+    {
+        //Semisphere
+        ( (x*y)+(y*y)+( (z-n)*(z-n) ) <= (r*r) && n <= z) 
+        
+        || 
+        
+        //Cylinder
+        ((x*x)+(y*y) <= (r*r) && 0<=z<=n)
+    }
+
+    function verifySemisphere(x:int, y:int, z:int) : bool
+    reads this`r, this`n
+    {
+        (x*x)+(y*y)+((z-n)*(z-n)) <= (r*r) && n <= z
+    }
+
+    function verifyIdle() : bool
+    reads this`z, this`curSpeed
+    {
+        z != 0 && curSpeed == 0
     }
     
-    function Moving():bool
-
-    function Landed():bool
-    ensures point.z==0.0
+    function verifyMoving():bool
+    reads this`z, this`curSpeed, this`maxSpeed
     {
-       
+        curSpeed == maxSpeed
+    }
+
+    function verifyLanded():bool
+    reads this`z, this`curSpeed
+    {
+        z == 0 && curSpeed == 0
     }
     
     
 
-    function Patrolling():bool 
-    
-    function Hovering():bool 
-
-    method move()
+    function verifyPatrolling():bool 
+    reads this`x, this`y, this`z, this`r, this`n, this`curSpeed, this`maxSpeed
     {
+        curSpeed == (maxSpeed/2)
+
+        &&
+
+        verifySemisphere(x,y,z)
+    }
+    
+
+/*
+    method getX() returns (x:int)
+    {
+        return x;
+    }
+
+    method getY() returns (y:int){
+        return y;
+    }
+
+    method getZ() returns (z:int){
+        return z;
+    }
+*/
+
+    method move(x:int, y:int, z:int)
+    modifies this`targetX, this`targetY, this`targetZ, this`curSpeed
+    requires RepInv()
+    requires verifyIdle()
+    ensures RepInv()
+    ensures verifyMoving()
+    {
+        targetX := x;
+        targetY := y;
+        targetZ := z;
+        curSpeed := maxSpeed;
+
 
     }
 
     method completeMove()
+    requires RepInv()
+    ensures RepInv()
     {
 
     }
 
     method addWaypoint()
+    requires RepInv()
+    ensures RepInv()
     {
 
     }
 
     method nextWayPoint()
+    requires RepInv()
+    ensures RepInv()
     {
 
     }
 
     method takeOff()
+    requires RepInv()
+    ensures RepInv()
     {
 
     }
 
     method completeTakeOff()
+    requires RepInv()
+    ensures RepInv()
     {
 
     }
 
     method land()
+    requires RepInv()
+    ensures RepInv()
     {
 
     }
 
     method completeLand()
+    requires RepInv()
+    ensures RepInv()
     {
 
     }
